WIP on generalization

theories/ftlr_bin_ctxt_ref.v
@@ -1,213 +1,383 @@
+From iris.algebra Require Import auth agree excl gmap frac.
 From iris.proofmode Require Import proofmode environments.
 From iris.program_logic Require Export weakestpre.
 From iris Require Import adequacy.
+
 From cap_machine Require Import linking logrel_binary.
 From cap_machine Require Import stdpp_restrict iris_extra.
 From cap_machine Require Import fundamental_binary contextual_refinement.
 From cap_machine Require Import machine_run.
 
 Section logrel.
-  Context {Σ:gFunctors} {memg:memG Σ} {regg:regG Σ}
-          {nainv: logrel_na_invs Σ} {cfgsg: cfgSG Σ}
-          {MP:MachineParameters}.
-
   Context {Symbols:Type}.
   Context {Symbols_eq_dec: EqDecision Symbols}.
   Context {Symbols_countable: Countable Symbols}.
+
+  Context {Σ: gFunctors}.
+  Context {MP: MachineParameters}.
 
   Local Coercion segment : component >-> segment_type.
 
   Notation "b |ᵣ a" := (restrict_map (a : gmap _ _) (b : gmap _ _)) (at level 80).
   Infix "##ₗ" := (can_link can_address_only_no_seals) (at level 70).
 
-  (** Lifting the interp binary value relation from words to components
-      This implies dom (exports y) ⊆ dom (exports x) *)
-  Definition interp_exports (x y: component Symbols) : iProp Σ :=
-    [∗ map] s ↦ wy ∈ exports y,
-        match exports x !! s with
-        | None => False (* values exported by y must also be exported by x *)
-        | Some wx =>
-          (* ([∗ map] a ↦ w ∈ segment x, a ↦ₐ w) ∗
-          ([∗ map] a ↦ w ∈ segment y, a ↣ₐ w) -∗ *)
-            interp (wx, wy)
-        end.
+  Section interp_exports.
+    Context {memg:memG Σ}.
+    Context {regg:regG Σ}.
+    Context {nainv: logrel_na_invs Σ}.
+    Context {cfgsg: cfgSG Σ}.
 
-  (** Allocates invariants for segment c in links (x ⋈ c) and (y ⋈ c)
-      assuming the exports of x and y are valid. *)
-  Lemma interp_exports_inv_alloc E {x y c: component Symbols} :
-    (∀ w, w ∈ img (segment c) -> is_int w) ->
-    x ##ₗ c -> y ##ₗ c ->
-    dom (exports x) ⊆ dom (exports y) ->
-    ([∗ map] a ↦ w ∈ x ⋈ c |ᵣ c, a ↦ₐ w) ∗
-    ([∗ map] a ↦ w ∈ y ⋈ c |ᵣ c, a ↣ₐ w) ∗
-    interp_exports x y ={E}=∗
-      ([∗ map] a ↦ _ ∈ c, inv (logN.@a) (interp_ref_inv a interp)).
-  Proof.
-    iIntros (Hno_caps Hsep1 Hsep2 Hexp) "[Hpx [Hpy #Hexp]]".
-    rewrite big_sepM_dom.
-    assert (Hdc:
-      dom (segment c) =
-      dom (map_zip (x ⋈ c : segment_type) (y ⋈ c: segment_type) |ᵣ c)).
-    { rewrite dom_restrict_map_L dom_map_zip_with_L -!(link_segment_dom can_address_only_no_seals).
-      set_solver. all: solve_can_link. }
-    rewrite Hdc -big_sepM_dom.
-    (* rewrite -(big_sepM_filter (fun '(a,_) => a ∈ _)). *)
-    rewrite (big_sepM_big_sepL2_map_to_list (fun a _ => inv _ _)).
-    iApply region_inv_alloc.
-    rewrite -(big_sepM_big_sepL2_map_to_list (fun a v => (a ↦ₐ v.1 ∗ a ↣ₐ v.2 ∗ interp v)%I)).
-    iApply (big_sepM_mono (fun a w =>
-      interp_exports x y ∗
-      (⌜ (x ⋈ c |ᵣ c) !! a = Some w.1 ⌝ ∗ a ↦ₐ w.1) ∗
-      (⌜ (y ⋈ c |ᵣ c) !! a = Some w.2 ⌝ ∗ a ↣ₐ w.2))%I).
-    iIntros (a [w w'] Hzip) "[#Hexp [[%Hxca Hw] [%Hyca Hw']]]".
-    simpl. iFrame.
-    (* assert validity of w,w' by case disjunction *)
-    apply map_filter_lookup_Some in Hxca as [Hxca Ha].
-    apply map_filter_lookup_Some in Hyca as [Hyca _]. apply elem_of_dom in Ha.
-    rewrite (link_segment_lookup_r _ Hsep1 Ha) in Hxca.
-    rewrite (link_segment_lookup_r _ Hsep2 Ha) in Hyca.
-    rewrite !resolve_imports_spec /= in Hxca, Hyca.
-    destruct (imports c !! a) as [s|] eqn:Hic.
-    destruct (exports y !! s) as [wy|] eqn:Hey;
-    destruct (exports x !! s) as [wx|] eqn:Hex.
-    apply Some_inj in Hxca, Hyca.
-    (* if they are exports from x,y, validity comes from the hypothese *)
-    1,2: iPoseProof (big_sepM_lookup _ _ _ _ Hey with "Hexp") as "H".
-    rewrite Hex Hxca Hyca. iApply "H".
-    rewrite Hex. done.
-    apply mk_is_Some, elem_of_dom in Hex.
-    apply not_elem_of_dom in Hey.
-    contradiction (Hey (Hexp _ Hex)).
-    (* else we know they are only words, and thus valid *)
-    1,2: rewrite Hxca in Hyca; apply Some_inj in Hyca; rewrite -Hyca.
-    1,2: apply (elem_of_map_img_2 (SA:=gset _)) in Hxca; apply Hno_caps in Hxca; unfold is_int in Hxca.
-    1,2: destruct w as [z | sb | z sb];
-         [ (rewrite fixpoint_interp1_eq; done) | | ];
-         destruct sb; simpl in Hxca; discriminate Hxca.
+    (** Lifting the interp binary value relation from words to components
+        This implies dom (exports y) ⊆ dom (exports x) *)
+    Definition interp_exports (x y: component Symbols) : iProp Σ :=
+      [∗ map] s ↦ wy ∈ exports y,
+          match exports x !! s with
+          | None => False (* values exported by y must also be exported by x *)
+          | Some wx =>
+            (* ([∗ map] a ↦ w ∈ segment x, a ↦ₐ w) ∗
+            ([∗ map] a ↦ w ∈ segment y, a ↣ₐ w) -∗ *)
+              interp (wx, wy)
+          end.
 
-    rewrite (big_sepM_sep (fun _ _ => interp_exports x y)).
-    iSplitR.
-    iApply big_sepM_dup. iModIntro. iIntros "H".
-    iFrame. done. done. unfold restrict_map.
-    rewrite restrict_map_zip_with.
-    iApply (big_sepM_sep_zip_affine
-      (fun a v => a ↦ₐ v)%I
-      (fun a v => a ↣ₐ v)%I).
-    iFrame.
+    (** Allocates invariants for segment c in links (x ⋈ c) and (y ⋈ c)
+        assuming the exports of x and y are valid. *)
+    Lemma interp_exports_inv_alloc E {x y c: component Symbols} :
+      (∀ w, w ∈ img (segment c) -> is_int w) ->
+      x ##ₗ c -> y ##ₗ c ->
+      dom (exports x) ⊆ dom (exports y) ->
+      ([∗ map] a ↦ w ∈ x ⋈ c |ᵣ c, a ↦ₐ w) ∗
+      ([∗ map] a ↦ w ∈ y ⋈ c |ᵣ c, a ↣ₐ w) ∗
+      interp_exports x y ={E}=∗
+        ([∗ map] a ↦ _ ∈ c, inv (logN.@a) (interp_ref_inv a interp)).
+    Proof.
+      iIntros (Hno_caps Hsep1 Hsep2 Hexp) "[Hpx [Hpy #Hexp]]".
+      rewrite big_sepM_dom.
+      assert (Hdc:
+        dom (segment c) =
+        dom (map_zip (x ⋈ c : segment_type) (y ⋈ c: segment_type) |ᵣ c)).
+      { rewrite dom_restrict_map_L dom_map_zip_with_L -!(link_segment_dom can_address_only_no_seals).
+        set_solver. all: solve_can_link. }
+      rewrite Hdc -big_sepM_dom.
+      (* rewrite -(big_sepM_filter (fun '(a,_) => a ∈ _)). *)
+      rewrite (big_sepM_big_sepL2_map_to_list (fun a _ => inv _ _)).
+      iApply region_inv_alloc.
+      rewrite -(big_sepM_big_sepL2_map_to_list (fun a v => (a ↦ₐ v.1 ∗ a ↣ₐ v.2 ∗ interp v)%I)).
+      iApply (big_sepM_mono (fun a w =>
+        interp_exports x y ∗
+        (⌜ (x ⋈ c |ᵣ c) !! a = Some w.1 ⌝ ∗ a ↦ₐ w.1) ∗
+        (⌜ (y ⋈ c |ᵣ c) !! a = Some w.2 ⌝ ∗ a ↣ₐ w.2))%I).
+      iIntros (a [w w'] Hzip) "[#Hexp [[%Hxca Hw] [%Hyca Hw']]]".
+      simpl. iFrame.
+      (* assert validity of w,w' by case disjunction *)
+      apply map_filter_lookup_Some in Hxca as [Hxca Ha].
+      apply map_filter_lookup_Some in Hyca as [Hyca _]. apply elem_of_dom in Ha.
+      rewrite (link_segment_lookup_r _ Hsep1 Ha) in Hxca.
+      rewrite (link_segment_lookup_r _ Hsep2 Ha) in Hyca.
+      rewrite !resolve_imports_spec /= in Hxca, Hyca.
+      destruct (imports c !! a) as [s|] eqn:Hic.
+      destruct (exports y !! s) as [wy|] eqn:Hey;
+      destruct (exports x !! s) as [wx|] eqn:Hex.
+      apply Some_inj in Hxca, Hyca.
+      (* if they are exports from x,y, validity comes from the hypothese *)
+      1,2: iPoseProof (big_sepM_lookup _ _ _ _ Hey with "Hexp") as "H".
+      rewrite Hex Hxca Hyca. iApply "H".
+      rewrite Hex. done.
+      apply mk_is_Some, elem_of_dom in Hex.
+      apply not_elem_of_dom in Hey.
+      contradiction (Hey (Hexp _ Hex)).
+      (* else we know they are only words, and thus valid *)
+      1,2: rewrite Hxca in Hyca; apply Some_inj in Hyca; rewrite -Hyca.
+      1,2: apply (elem_of_map_img_2 (SA:=gset _)) in Hxca; apply Hno_caps in Hxca; unfold is_int in Hxca.
+      1,2: destruct w as [z | sb | z sb];
+          [ (rewrite fixpoint_interp1_eq; done) | | ];
+          destruct sb; simpl in Hxca; discriminate Hxca.
 
-    Unshelve. typeclasses eauto.
-  Qed.
-
-  Lemma interp_link_exports {x y c:component Symbols}:
-    x ##ₗ c -> y ##ₗ c ->
-    spec_ctx ∗ interp_exports x y ∗
-    ([∗ map] a ↦ _ ∈ c, inv (logN.@a) (interp_ref_inv a interp)) -∗
-    interp_exports (x ⋈ c) (y ⋈ c).
-  Proof.
-    iIntros (Hsep1 Hsep2) "[#Hspec [#Hexp #Hinv]]".
-    (* weird induction scheme: essentially an induction on the exports of c
-       but keeping our persistent hypotheses out of the induction *)
-    apply (exports_ind (fun c' => envs_entails
-    (Envs
-    (Esnoc _ "Hinv"
-       ([∗ map] a ↦ _ ∈ c, inv _ (interp_ref_inv a interp)))
-    _ _)
-    _)%I c).
-    (* For exports from x,y this is a direct result of our hypothese *)
-    - iApply big_sepM_intro. iModIntro.
-      rewrite /= !map_union_empty. iIntros (s w) "%Hey".
-      iPoseProof (big_sepM_lookup _ _ _ _ Hey with "Hexp") as "H'".
-      destruct (exports x !! s); done.
-    (* For exports of c we need to do a bit of work.
-       First, prove they are indeed exports of c and not x or y *)
-    - iIntros (s w exp Hec Hexp Hexp_sub IH).
-      inversion Hsep1. inversion Hsep2. inversion Hwf_r.
-      destruct (exports y !! s) as [ey|] eqn:Hey.
-      rewrite map_disjoint_dom in Hexp_disj0.
-      apply mk_is_Some, elem_of_dom in Hec, Hey.
-      contradiction (Hexp_disj0 _ Hey Hec).
-      destruct (exports x !! s) as [ex|] eqn:Hex.
-      rewrite map_disjoint_dom in Hexp_disj.
-      apply mk_is_Some, elem_of_dom in Hec, Hex.
-      contradiction (Hexp_disj _ Hex Hec).
-      unfold interp_exports. iSimpl.
-      replace (exports y ∪ <[s:=w]> exp) with (<[s:=w]> (exports y ∪ exp)).
-      iApply big_sepM_insert. apply lookup_union_None. split; assumption.
+      rewrite (big_sepM_sep (fun _ _ => interp_exports x y)).
       iSplitR.
-      (* Now use the invariants to prove the validity of these exports *)
-      + rewrite (lookup_union_r _ _ _ Hex) lookup_insert.
-        rewrite fixpoint_interp1_eq.
-        destruct w. done.
-        destruct sb.
-        2,3: specialize (Hwr_exp _ (elem_of_map_img_2 _ _ _ Hec));
-             destruct s0; contradiction Hwr_exp.
-        destruct p. done.
-        all: iSplitR; [done|].
-        (* Use fundamental theorem to change interp_expr into interp *)
-        4: iIntros (r); do 2 iModIntro; iApply fundamental_binary;
-           done || rewrite fixpoint_interp1_eq; iSimpl; iSplitR; try done.
-        (* add the hypothese a ∈ dom (segment c) which we need to access our invariants *)
-        all: iApply (big_sepL_mono (fun _ a => ⌜a ∈ dom (segment c)⌝ -∗ _)%I);
-             [ (iIntros (k y' Hk) "Hl"; iApply "Hl"; iPureIntro;
-                apply (Hwr_exp _ (elem_of_map_img_2 _ _ _ Hec)), elem_of_finz_seq_between, elem_of_list_lookup;
-                exists k; apply Hk) | ].
-        all: induction (finz.seq_between f f0);
-             [ (iApply big_sepL_nil; done) |].
-        all: iApply big_sepL_cons; iSplitR; [ | apply IHl].
-        all: iIntros "%Ha"; iExists interp.
-        (* read_cond and write_cond boil down to interp -> interp,
-           so they are trivial *)
-        all: iSplitL;
-             [ | (try iSplitL; iSimpl; do 2 iModIntro; iIntros (ww ww') "H"; done)].
-        (* others results come from the invariants *)
-        all: apply elem_of_dom in Ha as [z Ha].
-        all: iPoseProof (big_sepM_lookup _ _ a _ Ha with "Hinv") as "Ha0".
-        all: iApply "Ha0"; iPureIntro; exact Ha.
-      + unfold interp_exports in IH. simpl in IH.
-        iApply (big_sepM_mono (fun k wy =>
-          interp_exports x y ∗ match (exports x ∪ exp) !! k with
-            | Some wx => interp (wx, wy)
-            | None => False%I
-          end)%I (fun k wy =>
-          match (exports x ∪ <[s:=w]> exp) !! k with
-            | Some wx => interp (wx, wy)
-            | None => False%I
-          end) (exports y ∪ exp)).
-        iIntros (s' wy Hwy) "[#Hexp #H]".
-        apply lookup_union_Some_raw in Hwy as [Hwy | [Hwy Hexp_y] ].
-        iPoseProof (big_sepM_lookup _ _ _ _ Hwy with "Hexp") as "H'".
-        destruct (exports x !! s') eqn:Hx.
-        rewrite !(lookup_union_Some_l _ _ _ _ Hx). done. done.
-        destruct (exports x !! s') eqn:Hx.
-        rewrite map_subseteq_spec in Hexp_sub.
-        rewrite map_disjoint_spec in Hexp_disj.
-        contradiction (Hexp_disj s' _ _ Hx (Hexp_sub s' _ Hexp_y)).
-        destruct (decide (s=s')) as [Heq|Heq].
-        rewrite Heq in Hexp. rewrite Hexp in Hexp_y. discriminate.
-        rewrite !(lookup_union_r _ _ _ Hx).
-        rewrite (lookup_insert_ne _ _ _ _ Heq). done.
-        iApply big_sepM_sep. iSplitR.
-        iApply big_sepM_intro. iModIntro. iIntros (k x0) "_". done.
-        apply IH.
-      + apply insert_union_r. assumption.
+      iApply big_sepM_dup. iModIntro. iIntros "H".
+      iFrame. done. done. unfold restrict_map.
+      rewrite restrict_map_zip_with.
+      iApply (big_sepM_sep_zip_affine
+        (fun a v => a ↦ₐ v)%I
+        (fun a v => a ↣ₐ v)%I).
+      iFrame.
 
-    Unshelve. all: typeclasses eauto.
-  Qed.
+      Unshelve. typeclasses eauto.
+    Qed.
 
-  Lemma interp_link E {x y c: component Symbols} :
-    (∀ w, w ∈ img (segment c) -> is_int w) ->
-    x ##ₗ c -> y ##ₗ c ->
-    dom (exports x) ⊆ dom (exports y) ->
-    spec_ctx ∗ interp_exports x y ∗
-    ([∗ map] a ↦ w ∈ x ⋈ c |ᵣ c, a ↦ₐ w) ∗
-    ([∗ map] a ↦ w ∈ y ⋈ c |ᵣ c, a ↣ₐ w) ={E}=∗
-    interp_exports (x ⋈ c) (y ⋈ c).
-  Proof.
-    iIntros (Hno_caps Hsep1 Hsep2 Hdom_incl) "(#Hspec & #Hxy & Hx & Hy)".
-    iApply (interp_link_exports Hsep1 Hsep2).
-    iSplitR. done. iSplitR. done.
-    iApply (interp_exports_inv_alloc E Hno_caps Hsep1 Hsep2 Hdom_incl).
-    iFrame. done.
-  Qed.
+    Lemma interp_link_exports {x y c:component Symbols}:
+      x ##ₗ c -> y ##ₗ c ->
+      spec_ctx ∗ interp_exports x y ∗
+      ([∗ map] a ↦ _ ∈ c, inv (logN.@a) (interp_ref_inv a interp)) -∗
+      interp_exports (x ⋈ c) (y ⋈ c).
+    Proof.
+      iIntros (Hsep1 Hsep2) "[#Hspec [#Hexp #Hinv]]".
+      (* weird induction scheme: essentially an induction on the exports of c
+        but keeping our persistent hypotheses out of the induction *)
+      apply (exports_ind (fun c' => envs_entails
+      (Envs
+      (Esnoc _ "Hinv"
+        ([∗ map] a ↦ _ ∈ c, inv _ (interp_ref_inv a interp)))
+      _ _)
+      _)%I c).
+      (* For exports from x,y this is a direct result of our hypothese *)
+      - iApply big_sepM_intro. iModIntro.
+        rewrite /= !map_union_empty. iIntros (s w) "%Hey".
+        iPoseProof (big_sepM_lookup _ _ _ _ Hey with "Hexp") as "H'".
+        destruct (exports x !! s); done.
+      (* For exports of c we need to do a bit of work.
+        First, prove they are indeed exports of c and not x or y *)
+      - iIntros (s w exp Hec Hexp Hexp_sub IH).
+        inversion Hsep1. inversion Hsep2. inversion Hwf_r.
+        destruct (exports y !! s) as [ey|] eqn:Hey.
+        rewrite map_disjoint_dom in Hexp_disj0.
+        apply mk_is_Some, elem_of_dom in Hec, Hey.
+        contradiction (Hexp_disj0 _ Hey Hec).
+        destruct (exports x !! s) as [ex|] eqn:Hex.
+        rewrite map_disjoint_dom in Hexp_disj.
+        apply mk_is_Some, elem_of_dom in Hec, Hex.
+        contradiction (Hexp_disj _ Hex Hec).
+        unfold interp_exports. iSimpl.
+        replace (exports y ∪ <[s:=w]> exp) with (<[s:=w]> (exports y ∪ exp)).
+        iApply big_sepM_insert. apply lookup_union_None. split; assumption.
+        iSplitR.
+        (* Now use the invariants to prove the validity of these exports *)
+        + rewrite (lookup_union_r _ _ _ Hex) lookup_insert.
+          rewrite fixpoint_interp1_eq.
+          destruct w. done.
+          destruct sb.
+          2,3: specialize (Hwr_exp _ (elem_of_map_img_2 _ _ _ Hec));
+              destruct s0; contradiction Hwr_exp.
+          destruct p. done.
+          all: iSplitR; [done|].
+          (* Use fundamental theorem to change interp_expr into interp *)
+          4: iIntros (r); do 2 iModIntro; iApply fundamental_binary;
+            done || rewrite fixpoint_interp1_eq; iSimpl; iSplitR; try done.
+          (* add the hypothese a ∈ dom (segment c) which we need to access our invariants *)
+          all: iApply (big_sepL_mono (fun _ a => ⌜a ∈ dom (segment c)⌝ -∗ _)%I);
+              [ (iIntros (k y' Hk) "Hl"; iApply "Hl"; iPureIntro;
+                  apply (Hwr_exp _ (elem_of_map_img_2 _ _ _ Hec)), elem_of_finz_seq_between, elem_of_list_lookup;
+                  exists k; apply Hk) | ].
+          all: induction (finz.seq_between f f0);
+              [ (iApply big_sepL_nil; done) |].
+          all: iApply big_sepL_cons; iSplitR; [ | apply IHl].
+          all: iIntros "%Ha"; iExists interp.
+          (* read_cond and write_cond boil down to interp -> interp,
+            so they are trivial *)
+          all: iSplitL;
+              [ | (try iSplitL; iSimpl; do 2 iModIntro; iIntros (ww ww') "H"; done)].
+          (* others results come from the invariants *)
+          all: apply elem_of_dom in Ha as [z Ha].
+          all: iPoseProof (big_sepM_lookup _ _ a _ Ha with "Hinv") as "Ha0".
+          all: iApply "Ha0"; iPureIntro; exact Ha.
+        + unfold interp_exports in IH. simpl in IH.
+          iApply (big_sepM_mono (fun k wy =>
+            interp_exports x y ∗ match (exports x ∪ exp) !! k with
+              | Some wx => interp (wx, wy)
+              | None => False%I
+            end)%I (fun k wy =>
+            match (exports x ∪ <[s:=w]> exp) !! k with
+              | Some wx => interp (wx, wy)
+              | None => False%I
+            end) (exports y ∪ exp)).
+          iIntros (s' wy Hwy) "[#Hexp #H]".
+          apply lookup_union_Some_raw in Hwy as [Hwy | [Hwy Hexp_y] ].
+          iPoseProof (big_sepM_lookup _ _ _ _ Hwy with "Hexp") as "H'".
+          destruct (exports x !! s') eqn:Hx.
+          rewrite !(lookup_union_Some_l _ _ _ _ Hx). done. done.
+          destruct (exports x !! s') eqn:Hx.
+          rewrite map_subseteq_spec in Hexp_sub.
+          rewrite map_disjoint_spec in Hexp_disj.
+          contradiction (Hexp_disj s' _ _ Hx (Hexp_sub s' _ Hexp_y)).
+          destruct (decide (s=s')) as [Heq|Heq].
+          rewrite Heq in Hexp. rewrite Hexp in Hexp_y. discriminate.
+          rewrite !(lookup_union_r _ _ _ Hx).
+          rewrite (lookup_insert_ne _ _ _ _ Heq). done.
+          iApply big_sepM_sep. iSplitR.
+          iApply big_sepM_intro. iModIntro. iIntros (k x0) "_". done.
+          apply IH.
+        + apply insert_union_r. assumption.
 
+      Unshelve. all: typeclasses eauto.
+    Qed.
+
+    Lemma interp_link E {x y c: component Symbols} :
+      (∀ w, w ∈ img (segment c) -> is_int w) ->
+      x ##ₗ c -> y ##ₗ c ->
+      dom (exports x) ⊆ dom (exports y) ->
+      spec_ctx ∗ interp_exports x y ∗
+      ([∗ map] a ↦ w ∈ x ⋈ c |ᵣ c, a ↦ₐ w) ∗
+      ([∗ map] a ↦ w ∈ y ⋈ c |ᵣ c, a ↣ₐ w) ={E}=∗
+      interp_exports (x ⋈ c) (y ⋈ c).
+    Proof.
+      iIntros (Hno_caps Hsep1 Hsep2 Hdom_incl) "(#Hspec & #Hxy & Hx & Hy)".
+      iApply (interp_link_exports Hsep1 Hsep2).
+      iSplitR. done. iSplitR. done.
+      iApply (interp_exports_inv_alloc E Hno_caps Hsep1 Hsep2 Hdom_incl).
+      iFrame. done.
+    Qed.
+
+    Definition ctx_points_to γc (l_comp r_comp : component Symbols) (reg : Reg) : iProp Σ :=
+      ([∗ map] a↦w ∈ l_comp, a ↦ₐ w) ∗
+      ([∗ map] a↦w ∈ r_comp, a ↣ₐ w) ∗
+      ([∗ map] r↦w ∈ reg, r ↦ᵣ w) ∗
+      ([∗ map] r↦w ∈ reg, r ↣ᵣ w) ∗
+      na_own logrel_nais ⊤ ∗
+      own γc (◯ ((Excl' (Seq (Instr Executable)) : optionUR (exclR (leibnizO expr)), (∅,∅)) : cfgUR)) ∗
+      spec_res (Seq (Instr Executable)) (reg, segment r_comp).
+  End interp_exports.
+
+  Definition initial_state (c: component Symbols) (r:Reg): cfg cap_lang :=
+    ([Seq (Instr Executable)], (r, segment c)).
+
+  Section refinement.
+    Context {inv_preg: invGpreS Σ}.
+    Context {mem_preg: gen_heapGpreS Addr Word Σ}.
+    Context {reg_preg: gen_heapGpreS RegName Word Σ}.
+    Context {seal_store_preg: sealStorePreG Σ}.
+    Context {na_invg: na_invG Σ}.
+
+    (** Lemma to allocate memory and register map *)
+    Lemma regspec_mapsto_alloc `{cfgSG Σ} e (σ : gmap RegName Word * gmap Addr Word) r (w : Word) :
+      σ.1 !! r = None →
+      spec_res e σ ==∗ spec_res e (<[r:=w]> σ.1,σ.2) ∗ r ↣ᵣ w.
+    Proof.
+      iIntros (Hnone) "Hσ".
+      rewrite /spec_res /regspec_mapsto.
+      iMod (own_update with "Hσ") as "[Hσ Hr]".
+      { eapply auth_update_alloc,prod_local_update_2,prod_local_update_1.
+        eapply (alloc_singleton_local_update (to_spec_map σ.1) r (1%Qp, to_agree w)).
+        by rewrite lookup_fmap Hnone. done. }
+      iModIntro. iFrame "Hr". rewrite -fmap_insert. iFrame.
+    Qed.
+    Lemma memspec_mapsto_alloc `{cfgSG Σ} e (σ : gmap RegName Word * gmap Addr Word) a (w : Word) :
+      σ.2 !! a = None →
+      spec_res e σ ==∗ spec_res e (σ.1,<[a:=w]> σ.2) ∗ a ↣ₐ w.
+    Proof.
+      iIntros (Hnone) "Hσ".
+      rewrite /spec_res /memspec_mapsto.
+      iMod (own_update with "Hσ") as "[Hσ Hr]".
+      { eapply auth_update_alloc,prod_local_update_2,prod_local_update_2.
+        eapply (alloc_singleton_local_update (to_spec_map σ.2) a (1%Qp, to_agree w)).
+        by rewrite lookup_fmap Hnone. done. }
+      iModIntro. iFrame "Hr". rewrite -fmap_insert. iFrame.
+    Qed.
+    Lemma regspec_alloc_big `{cfgSG Σ} e σ σ' σs :
+      σ' ##ₘ σ →
+      spec_res e (σ,σs) ==∗
+      spec_res e (σ' ∪ σ,σs) ∗ ([∗ map] l ↦ v ∈ σ', l ↣ᵣ v).
+    Proof.
+      revert σ; induction σ' as [| l v σ' Hl IH] using map_ind; iIntros (σ Hdisj) "Hσ".
+      { rewrite left_id_L. auto. }
+      iMod (IH with "Hσ") as "[Hσ'σ Hσ']"; first by eapply map_disjoint_insert_l.
+      decompose_map_disjoint.
+      rewrite !big_opM_insert // -insert_union_l //.
+      iMod (regspec_mapsto_alloc with "Hσ'σ") as "($ & $)".
+        by apply lookup_union_None. done.
+    Qed.
+    Lemma memspec_alloc_big `{cfgSG Σ} e σ σ' σr :
+      σ' ##ₘ σ →
+      spec_res e (σr, σ) ==∗
+      spec_res e (σr, map_union σ' σ) ∗ ([∗ map] l ↦ v ∈ σ', l ↣ₐ v).
+    Proof.
+      revert σ; induction σ' as [| l v σ' Hl IH] using map_ind; iIntros (σ Hdisj) "Hσ".
+      { rewrite left_id_L. auto. }
+      iMod (IH with "Hσ") as "[Hσ'σ Hσ']"; first by eapply map_disjoint_insert_l.
+      decompose_map_disjoint.
+      rewrite !big_opM_insert //.
+      assert (map_union (<[l:=v]> σ') σ = <[l:=v]> (map_union σ' σ)) as ->.
+      { rewrite insert_union_l. auto. }
+      iMod (memspec_mapsto_alloc with "Hσ'σ") as "($ & $)".
+      simpl. rewrite lookup_union_None//. done.
+    Qed.
+
+    Context {cfgg : inG Σ (authR cfgUR)}.
+
+    Definition fat_hypothesis (l_comp r_comp : component Symbols) r :=
+      ∀ Hinv mem_heapg reg_heapg γc logrel_nais,
+      let memg := MemG Σ Hinv mem_heapg in
+      let regg := RegG Σ Hinv reg_heapg in
+      let logrel_na_invs := Build_logrel_na_invs Σ na_invg logrel_nais  in
+      let Hcfg := CFGSG Σ cfgg γc in
+      @ctx_points_to memg regg logrel_na_invs Hcfg γc l_comp r_comp r ={⊤}=∗
+      WP Seq (Instr Executable)
+      {{ v,
+         ⌜v = HaltedV⌝
+         → ∃ r0 : Reg * Reg, ⤇
+             of_val HaltedV ∗
+             full_map r0
+             ∧ registers_mapsto r0.1 ∗
+             spec_registers_mapsto r0.2 ∗
+             na_own logrel.logrel_nais ⊤ }} ∗
+      inv specN (spec_inv ([Seq (Instr Executable)], (r, segment r_comp))).
+
+      (* @interp_exports memg regg logrel_na_invs Hcfg l_comp r_comp. *)
+
+    Lemma interp_refinement (comp_l comp_r : component Symbols) r conf  :
+      fat_hypothesis comp_l comp_r r ->
+      rtc erased_step (initial_state comp_l r) ([of_val HaltedV], conf) ->
+      (∃ conf', rtc erased_step (initial_state comp_r r) ([of_val HaltedV], conf')).
+    Proof.
+      intros Hfat Hstep.
+      cut (@adequate cap_lang NotStuck
+              (Seq (Instr Executable))
+              (r, segment comp_l)
+              (λ v _, v = HaltedV → ∃ conf',
+                rtc erased_step
+                  (initial_state comp_r r)
+                  ([of_val HaltedV], conf'))).
+      { intros [adequate_result _]. apply adequate_result in Hstep; [ apply Hstep | done ]. }
+      eapply (wp_adequacy Σ _).
+      iIntros (Hinv κs).
+
+      iMod (gen_heap_init (segment comp_l:Mem)) as (mem_heapg) "(Hmem_ctx & Hmem & _)".
+      iMod (gen_heap_init (r:Reg)) as (reg_heapg) "(Hreg_ctx & Hreg & _)".
+      iMod (seal_store_init) as (seal_storeg) "Hseal_store".
+      iMod (@na_alloc Σ na_invg) as (logrel_nais) "Hna".
+
+      iMod (own_alloc (● (Excl' (Seq (Instr Executable)) : optionUR (exclR (leibnizO expr)), (∅,∅))
+                        ⋅ ◯ ((Excl' (Seq (Instr Executable)) : optionUR (exclR (leibnizO expr)), (∅,∅)) : cfgUR)))
+        as (γc) "[Hcfg1 Hcfg2]".
+      { apply auth_both_valid_discrete. split=>//. }
+
+      pose memg := MemG Σ Hinv mem_heapg.
+      pose regg := RegG Σ Hinv reg_heapg.
+      pose logrel_na_invs := Build_logrel_na_invs _ na_invg logrel_nais.
+      pose Hcfg := CFGSG _ _ γc.
+
+      iMod (regspec_alloc_big _ ∅ r ∅ with "[Hcfg1]") as "(Hcfg1 & Hregspec)".
+        by apply map_disjoint_empty_r.
+        rewrite /spec_res /= !/to_spec_map !fmap_empty //.
+      rewrite right_id_L.
+      iMod (memspec_alloc_big _ ∅ (segment comp_r) r with "[Hcfg1]") as "(Hcfg1 & Hmemspec)".
+        by apply map_disjoint_empty_r. rewrite /spec_res /= !/to_spec_map !fmap_empty //.
+      rewrite right_id_L.
+
+      specialize (Hfat Hinv mem_heapg reg_heapg γc logrel_nais).
+      simpl in Hfat.
+      iPoseProof (Hfat with "[Hmem Hmemspec Hreg Hregspec Hna Hcfg2 Hcfg1]") as ">[Hfat #Hspec]".
+      { iFrame. }
+
+      iModIntro.
+      iExists (fun σ κs => ((gen_heap_interp σ.1) ∗ (gen_heap_interp σ.2)))%I.
+      iExists (fun _ => True)%I. iFrame.
+      iApply wp_fupd. iApply wp_wand_r. iFrame.
+
+      iIntros (v) "Hcond".
+      destruct v;[|iModIntro;iIntros (Hcontr);done..].
+      iDestruct ("Hcond" $! eq_refl) as (r') "(Hj & Hcond)".
+      iInv specN as ">Hres" "Hcls". iDestruct "Hres" as (e' σ') "[Hown Hsteps]".
+      iDestruct "Hsteps" as %Hsteps.
+      iDestruct (own_valid_2 with "Hown Hj") as %Hvalid.
+      iMod ("Hcls" with "[Hown]") as "_".
+      { iNext. iExists _,_. eauto. }
+      iModIntro.
+      apply auth_both_valid_discrete in Hvalid as [Hincl Hvalid].
+      iIntros (_).
+      apply prod_included in Hincl as [Hincl Hincl']. simpl in *.
+      revert Hincl; rewrite Excl_included =>Hincl.
+      apply leibniz_equiv in Hincl as <-.
+      iExists σ'. iPureIntro. apply Hsteps.
+    Qed.
+  End refinement.
 End logrel.
